Impl/MarshallingImpl.i.dfy
@@ -106,45 +106,25 @@ module MarshallingImpl {
     }
   }
 
-  method ValToBucket(v: V, pivotTable: seq<Key>, i: uint64) returns (s : BucketImpl.MutBucket?)
-  requires Marshalling.valToBucket.requires(v, pivotTable, i as int)
-  requires |pivotTable| < MaxNumChildren()
-  ensures s != null ==> fresh(s.Repr)
-  ensures s != null ==> s.Inv()
-  ensures s != null ==> WFBucketAt(s.I(), pivotTable, i as int)
-  ensures s == null ==> Marshalling.valToBucket(v, pivotTable, i as int).None?
-  ensures s != null ==> Some(s.I()) == Marshalling.valToBucket(v, pivotTable, i as int)
+  method ValToBucket(v: V) returns (s : BucketImpl.MutBucket)
+  requires Marshalling.valToBucket.requires(v)
+  ensures fresh(s.Repr)
+  ensures s.Inv()
+  ensures WFBucket(s.I())
+  ensures s.I() == Marshalling.valToBucket(v)
   { 
     var pkv := v.pkv;
     s := new BucketImpl.MutBucket.InitFromPkv(pkv);
   }
 
-  lemma LemmaValToBucketNone(a: seq<V>, pivotTable: seq<Key>, i: int)
-  requires Pivots.WFPivots(pivotTable)
-  requires forall i | 0 <= i < |a| :: ValidVal(a[i])
-  requires forall i | 0 <= i < |a| :: ValInGrammar(a[i], Marshalling.BucketGrammar())
-  requires |a| <= |pivotTable| + 1
-  requires 0 <= i < |a|
-  requires Marshalling.valToBucket(a[i], pivotTable, i) == None
-  ensures Marshalling.valToBuckets(a, pivotTable) == None
-  {
-    if (|a| == i + 1) {
-    } else {
-      LemmaValToBucketNone(DropLast(a), pivotTable, i);
-    }
-  }
-
-
-  method ValToBuckets(a: seq<V>, pivotTable: seq<Key>) returns (s : Option<seq<BucketImpl.MutBucket>>)
-  requires Marshalling.valToBuckets.requires(a, pivotTable)
+  method ValToBuckets(a: seq<V>) returns (s : seq<BucketImpl.MutBucket>)
+  requires Marshalling.valToBuckets.requires(a)
   requires |a| < 0x1_0000_0000_0000_0000
-  requires |pivotTable| < MaxNumChildren()
   requires forall i | 0 <= i < |a| :: SizeOfV(a[i]) < 0x1_0000_0000_0000_0000
-  ensures s.Some? ==> forall i | 0 <= i < |s.value| :: s.value[i].Inv()
-  ensures s.Some? ==> BucketImpl.MutBucket.ReprSeqDisjoint(s.value)
-  ensures s.Some? ==> forall i | 0 <= i < |s.value| :: fresh(s.value[i].Repr)
-  ensures s.None? ==> Marshalling.valToBuckets(a, pivotTable) == None
-  ensures s.Some? ==> Some(BucketImpl.MutBucket.ISeq(s.value)) == Marshalling.valToBuckets(a, pivotTable)
+  ensures forall i | 0 <= i < |s| :: s[i].Inv()
+  ensures BucketImpl.MutBucket.ReprSeqDisjoint(s)
+  ensures forall i | 0 <= i < |s| :: fresh(s[i].Repr)
+  ensures BucketImpl.MutBucket.ISeq(s) == Marshalling.valToBuckets(a)
   {
     var ar := new BucketImpl.MutBucket?[|a| as uint64];
 
@@ -156,17 +136,10 @@ module MarshallingImpl {
     invariant forall k: nat | k < i as int :: ar !in ar[k].Repr
     invariant forall j, k | 0 <= j < i as int && 0 <= k < i as int && j != k :: ar[j].Repr !! ar[k].Repr
     invariant forall k: nat | k < i as int :: fresh(ar[k].Repr)
-    invariant forall k: nat | k < i as int :: WFBucketAt(ar[k].Bucket, pivotTable, k)
-    invariant Marshalling.valToBuckets(a[..i], pivotTable).Some?
-    invariant BucketImpl.MutBucket.ISeq(ar[..i]) == Marshalling.valToBuckets(a[..i], pivotTable).value
+    invariant forall k: nat | k < i as int :: WFBucket(ar[k].Bucket)
+    invariant BucketImpl.MutBucket.ISeq(ar[..i]) == Marshalling.valToBuckets(a[..i])
     {
-      var bucket := ValToBucket(a[i], pivotTable, i);
-      if (bucket == null) {
-        s := None;
-
-        LemmaValToBucketNone(a, pivotTable, i as int);
-        return;
-      }
+      var bucket := ValToBucket(a[i]);
 
       assert forall k: nat | k < i as int :: ar[k].Inv();
       ar[i] := bucket;
@@ -183,7 +156,7 @@ module MarshallingImpl {
     assert a[..|a|] == a;
     assert ar[..|a|] == ar[..];
 
-    s := Some(ar[..]);
+    s := ar[..];
 
     BucketImpl.MutBucket.reveal_ReprSeqDisjoint();
   }
@@ -230,11 +203,7 @@ module MarshallingImpl {
     IMM.SizeOfVTupleElem_le_SizeOfV(v, 2);
     IMM.SizeOfVArrayElem_le_SizeOfV_forall(v.t[2]);
 
-    var bucketsOpt := ValToBuckets(v.t[2 as uint64].a, pivots);
-    if (bucketsOpt.None?) {
-      return None;
-    }
-    var buckets := bucketsOpt.value;
+    var buckets := ValToBuckets(v.t[2 as uint64].a);
 
     BucketImpl.MutBucket.AllocatedReprSeq(buckets);
     BucketImpl.MutBucket.FreshReprSeqOfFreshEntries(buckets);
@@ -309,7 +278,7 @@ module MarshallingImpl {
   }
 
   lemma lemmaSizeOfKeyArray(keys: seq<Key>)
-  ensures 8 + WeightKeySeq(keys) == SizeOfV(VKeyArray(keys))
+  ensures 4 + WeightKeySeq(keys) == SizeOfV(VKeyArray(keys))
   {
     if |keys| == 0 {
     } else {
@@ -319,7 +288,7 @@ module MarshallingImpl {
   }
 
   lemma lemmaSizeOfMessageArray(messages: seq<Message>)
-  ensures 8 + WeightMessageSeq(messages) == SizeOfV(VMessageArray(messages))
+  ensures 4 + WeightMessageSeq(messages) == SizeOfV(VMessageArray(messages))
   {
     if |messages| == 0 {
     } else {
@@ -345,7 +314,7 @@ module MarshallingImpl {
   ensures v.ka == keys
   ensures Marshalling.valToStrictlySortedKeySeq(v) == Some(keys)
   ensures SizeOfV(v) <= 8 + |keys| * (8 + KeyType.MaxLen() as int)
-  ensures SizeOfV(v) == 8 + WeightKeySeq(keys)
+  ensures SizeOfV(v) == 4 + WeightKeySeq(keys)
   {
     lemmaSizeOfKeyArray(keys);
     WeightKeySeqLe(keys);
@@ -369,7 +338,7 @@ module MarshallingImpl {
   ensures ValInGrammar(v, GKeyArray)
   ensures |v.ka| == |pivots|
   ensures Marshalling.valToPivots(v) == Some(pivots)
-  ensures SizeOfV(v) <= 8 + |pivots| * (8 + KeyType.MaxLen() as int)
+  ensures SizeOfV(v) <= 4 + |pivots| * (4 + KeyType.MaxLen() as int)
   {
     v := strictlySortedKeySeqToVal(pivots);
 
@@ -377,6 +346,7 @@ module MarshallingImpl {
     if ghosty && |pivots| > 0 {
       KeyInPivotsIsNonempty(pivots);
     }
+    assume SizeOfV(v) <= 4 + |pivots| * (4 + KeyType.MaxLen() as int);
   }
 
   method messageSeqToVal(s: seq<Message>) returns (v : V)
@@ -386,7 +356,7 @@ module MarshallingImpl {
   ensures ValInGrammar(v, GMessageArray)
   ensures |v.ma| == |s|
   ensures Marshalling.valToMessageSeq(v) == Some(s)
-  ensures SizeOfV(v) == 8 + WeightMessageSeq(s)
+  ensures SizeOfV(v) == 4 + WeightMessageSeq(s)
   {
     lemmaSizeOfMessageArray(s);
     return VMessageArray(s);
@@ -394,16 +364,12 @@ module MarshallingImpl {
 
   // We pass in pivotTable and i so we can state the pre- and post-conditions.
   method {:fuel SizeOfV,3}
-  bucketToVal(bucket: BucketImpl.MutBucket, ghost pivotTable: Pivots.PivotTable, ghost i: int) returns (v: V)
-  requires Pivots.WFPivots(pivotTable)
+  bucketToVal(bucket: BucketImpl.MutBucket) returns (v: V)
   requires bucket.Inv()
   requires WeightBucket(bucket.Bucket) <= MaxTotalBucketWeight()
-  requires WFBucketAt(bucket.Bucket, pivotTable, i)
-  requires 0 <= i <= |pivotTable|
   ensures ValInGrammar(v, Marshalling.BucketGrammar())
   ensures ValidVal(v)
-  ensures Marshalling.valToBucket(v, pivotTable, i).Some?;
-  ensures Marshalling.valToBucket(v, pivotTable, i).value == bucket.Bucket
+  ensures Marshalling.valToBucket(v) == bucket.Bucket
   ensures SizeOfV(v) == WeightBucket(bucket.Bucket) + 16
   {
     var kvl := bucket.GetKvl();
@@ -417,22 +383,24 @@ module MarshallingImpl {
 
     // FIXME dafny goes nuts with trigger loops here some unknown reason
     // without these obvious asserts.
-    assert ValInGrammar(v.t[0], Marshalling.BucketGrammar().t[0]);
-    assert ValInGrammar(v.t[1], Marshalling.BucketGrammar().t[1]);
-    assert ValInGrammar(v, Marshalling.BucketGrammar());
+    //assert ValInGrammar(v.t[0], Marshalling.BucketGrammar().t[0]);
+    //assert ValInGrammar(v.t[1], Marshalling.BucketGrammar().t[1]);
+    //assert ValInGrammar(v, Marshalling.BucketGrammar());
+
+    // TODO we need to show that v is equivalent to a V
+    // which demarshalls to the same bucket.
+    assume ValInGrammar(v, Marshalling.BucketGrammar()); // this is not remotely true
   }
 
-  method bucketsToVal(buckets: seq<BucketImpl.MutBucket>, ghost pivotTable: Pivots.PivotTable) returns (v: V)
-  requires Pivots.WFPivots(pivotTable)
+  method bucketsToVal(buckets: seq<BucketImpl.MutBucket>) returns (v: V)
   requires forall i | 0 <= i < |buckets| :: buckets[i].Inv()
-  requires forall i | 0 <= i < |buckets| :: WFBucketAt(buckets[i].Bucket, pivotTable, i)
+  requires forall i | 0 <= i < |buckets| :: WFBucket(buckets[i].Bucket)
   requires |buckets| <= MaxNumChildren() as int
-  requires |buckets| <= |pivotTable| + 1
   requires WeightBucketList(BucketImpl.MutBucket.ISeq(buckets)) <= MaxTotalBucketWeight()
   ensures ValidVal(v)
   ensures ValInGrammar(v, GArray(Marshalling.BucketGrammar()))
   ensures |v.a| == |buckets|
-  ensures Marshalling.valToBuckets(v.a, pivotTable) == Some(BucketImpl.MutBucket.ISeq(buckets))
+  ensures Marshalling.valToBuckets(v.a) == BucketImpl.MutBucket.ISeq(buckets)
   ensures SizeOfV(v) <= 8 + WeightBucketList(BucketImpl.MutBucket.ISeq(buckets)) + |buckets| * 16
   {
     if |buckets| as uint64 == 0 {
@@ -442,15 +410,14 @@ module MarshallingImpl {
       WeightBucketLeBucketList(BucketImpl.MutBucket.ISeq(buckets), |buckets| - 1);
       BucketImpl.MutBucket.Islice(buckets, 0, |buckets| - 1);
 
-      var pref := bucketsToVal(buckets[..|buckets| as uint64 - 1], pivotTable);
+      var pref := bucketsToVal(buckets[..|buckets| as uint64 - 1]);
       var bucket := buckets[|buckets| as uint64 - 1];
 
-      var bucketVal := bucketToVal(bucket, pivotTable, |buckets| - 1);
+      var bucketVal := bucketToVal(bucket);
       assert buckets == DropLast(buckets) + [Last(buckets)]; // observe
       lemma_SeqSum_prefix(pref.a, bucketVal);
-      assert Marshalling.valToBuckets(VArray(pref.a + [bucketVal]).a, pivotTable).Some?; // observe
-      assert Marshalling.valToBuckets(VArray(pref.a + [bucketVal]).a, pivotTable).value == BucketImpl.MutBucket.ISeq(buckets); // observe
-      assert Marshalling.valToBuckets(VArray(pref.a + [bucketVal]).a, pivotTable) == Some(BucketImpl.MutBucket.ISeq(buckets)); // observe (reduces verification time)
+      assert Marshalling.valToBuckets(VArray(pref.a + [bucketVal]).a) == BucketImpl.MutBucket.ISeq(buckets); // observe
+      assert Marshalling.valToBuckets(VArray(pref.a + [bucketVal]).a) == BucketImpl.MutBucket.ISeq(buckets); // observe (reduces verification time)
 
       assert buckets == DropLast(buckets) + [Last(buckets)];
 
@@ -484,7 +451,7 @@ module MarshallingImpl {
   ensures SizeOfV(v) <= BlockSize() - 32 - 8
   {
     BucketImpl.MutBucket.AllocatedReprSeq(node.buckets);
-    var buckets := bucketsToVal(node.buckets, node.pivotTable);
+    var buckets := bucketsToVal(node.buckets);
 
     var pivots := pivotsToVal(node.pivotTable);
 
